# Antiderivative Solutions

## Problems 1–10

### 1. ∫ (2/3)x³ - 4x dx
**Solution:**  
∫ (2/3)x³ dx - ∫ 4x dx = (2/3)(x⁴/4) - 4(x²/2) = (1/6)x⁴ - 2x² + C  
**Answer:**  
(1/6)x⁴ - 2x² + C

---

### 2. ∫ (x + √x) dx  
**Solution:**  
√x = x^(1/2) ⇒ ∫ x dx + ∫ x^(1/2) dx = (1/2)x² + (2/3)x^(3/2) + C  
**Answer:**  
(1/2)x² + (2/3)x^(3/2) + C

---

### 3. ∫ (4 cos(4x) + 9 sin(3x)) dx  
**Solution:**  
= ∫ 4 cos(4x) dx + ∫ 9 sin(3x) dx  
= 4(1/4) sin(4x) - 9(1/3) cos(3x) + C  
= sin(4x) - 3 cos(3x) + C  
**Answer:**  
sin(4x) - 3 cos(3x) + C

---

### 4. ∫ (6 - x)/(5x) dx  
**Solution:**  
= (1/5) ∫ (6/x - 1) dx = (1/5)(6 ln|x| - x) + C  
**Answer:**  
(6 ln|x| - x)/5 + C

---

### 5. ∫ e^(-5x) dx  
**Solution:**  
= (1/-5) e^(-5x) + C  
**Answer:**  
(-1/5)e^(-5x) + C

---

### 6. ∫ (5 - x²)/x dx  
**Solution:**  
= ∫ 5/x dx - ∫ x dx = 5 ln|x| - (1/2)x² + C  
**Answer:**  
5 ln|x| - (1/2)x² + C

---

### 7. ∫ sec²(5x) dx  
**Solution:**  
= (1/5) tan(5x) + C  
**Answer:**  
(1/5) tan(5x) + C

---

### 8. ∫ sin(-3x) dx  
**Solution:**  
= -1/3 cos(-3x) + C = -1/3 cos(3x) + C  
**Answer:**  
(-1/3) cos(3x) + C

---

### 9. ∫ 5e^x dx  
**Solution:**  
= 5e^x + C  
**Answer:**  
5e^x + C

---

### 10. ∫ x√x dx  
**Solution:**  
= ∫ x * x^(1/2) dx = ∫ x^(3/2) dx = (2/5)x^(5/2) + C  
**Answer:**  
(2/5)x^(5/2) + C

---

## Problems 11–15 (Using Substitution)

### 11. ∫ (1 - x)^15 dx  
**Substitution:** u = 1 - x ⇒ du = -dx  
= -∫ u^15 du = -(u^16 / 16) + C = -((1 - x)^16 / 16) + C  
**Answer:**  
-((1 - x)^16) / 16 + C

---

### 12. ∫ (ln x)² / x dx  
**Substitution:** u = ln x ⇒ du = (1/x) dx  
= ∫ u² du = (u³ / 3) + C = (ln x)³ / 3 + C  
**Answer:**  
(ln x)³ / 3 + C

---

### 13. ∫ e^x * e^(e^x) dx  
**Substitution:** u = e^x ⇒ du = e^x dx  
= ∫ e^u du = e^u + C = e^(e^x) + C  
**Answer:**  
e^(e^x) + C

---

### 14. ∫ sin(x) * cos²(x) dx  
**Substitution:** u = cos(x) ⇒ du = -sin(x) dx  
= -∫ u² du = -(u³ / 3) + C = -(cos³(x)) / 3 + C  
**Answer:**  
-(cos³(x))/3 + C

---

### 15. ∫ (2x - 1) √(x² - x) dx  
**Substitution:** u = x² - x ⇒ du = (2x - 1) dx  
= ∫ √u du = ∫ u^(1/2) du = (2/3) u^(3/2) + C = (2/3)(x² - x)^(3/2) + C  
**Answer:**  
(2/3)(x² - x)^(3/2) + C

---
